backend/Conventions.v
@@ -186,6 +186,7 @@ Canonical Structure li_locset: language_interface :=
   {|
     query := locset_query;
     reply := locset_reply;
+    entry := lq_vf;
   |}.
 
 (** * Calling convention *)
@@ -198,12 +199,11 @@ Canonical Structure li_locset: language_interface :=
   registers can be enforced. *)
 
 Inductive cc_alloc_mq: signature * Locmap.t -> c_query -> locset_query -> Prop :=
-  cc_alloc_mq_intro vf1 vf2 sg args rs m1 m2:
-    Val.lessdef vf1 vf2 ->
+  cc_alloc_mq_intro vf sg args rs m1 m2:
     Val.lessdef_list args (map (fun p => Locmap.getpair p rs) (loc_arguments sg)) ->
     Mem.extends m1 m2 ->
     Val.has_type_list args (sig_args sg) ->
-    cc_alloc_mq (sg, rs) (cq vf1 sg args m1) (lq vf2 sg rs m2).
+    cc_alloc_mq (sg, rs) (cq vf sg args m1) (lq vf sg rs m2).
 
 Inductive cc_alloc_mr: signature * Locmap.t -> c_reply -> locset_reply -> Prop :=
   cc_alloc_mr_intro sg rs res rs' m1 m2:
@@ -223,11 +223,10 @@ Program Definition cc_alloc: callconv li_c li_locset :=
 (** The extension convention is used by the Tunneling proof. *)
 
 Inductive cc_locset_ext_query: locset_query -> locset_query -> Prop :=
-  cc_locset_ext_query_intro vf1 vf2 sg ls1 ls2 m1 m2:
-    Val.lessdef vf1 vf2 ->
+  cc_locset_ext_query_intro vf sg ls1 ls2 m1 m2:
     (forall l, Val.lessdef (ls1 l) (ls2 l)) ->
     Mem.extends m1 m2 ->
-    cc_locset_ext_query (lq vf1 sg ls1 m1) (lq vf2 sg ls2 m2).
+    cc_locset_ext_query (lq vf sg ls1 m1) (lq vf sg ls2 m2).
 
 Inductive cc_locset_ext_reply: locset_reply -> locset_reply -> Prop :=
   cc_locset_ext_reply_intro ls1 ls2 m1 m2:
